lean working stack

leanTheories/StackComp/OpWasm.lean
@@ -1,13 +1,54 @@
+/-!
+## Defining variables for the evaluation context
+- stack defines the list of values in the programs scopes
+-/
 def stack := List Int
 def empty_stack : List Int := []
 
-inductive binop: Type :=
+/-!
+# Defining operations for execution
+- **inst** represents instructions, as of right now they can be
+  - binary operations
+  - pushing constant values onto the stack
+
+## BNF notation and inference rules
+
+- Backus Naur Form to describe the **syntax**
+  - defined by `binop` and `inst`
+```
+        Instr := const Z
+          | binop
+
+        Binop := add
+          | minus
+          | mult
+          | div
+
+```
+
+- transition relations defined with inference rules to describe the **semantics**
+  - defined by `ieval` and `seval`
+
+```
+            
+                         st = [ x :: y :: sx ]
+          ---------------------------------------------------- (binary operation)
+             [x :: y :: sx] =[ (binop op) ]=> ([ (op x y) :: sx ])
+
+
+               --------------------------------------------- (Const)
+                      s =[ (Const 10) ] => 10 :: s
+```
+
+-/
+
+inductive binop: Type where
   | B_Add
   | B_Minus
   | B_Mult
   | B_Div
 
-inductive inst : Type :=
+inductive inst : Type where
   | Const (i: Int)
   | Binop (op : binop)
 
@@ -18,12 +59,13 @@ def bo_eval (op : binop) (x y : Int) : Int :=
   | .B_Mult => x * y
   | .B_Div => x / y
 
-inductive ieval : inst → stack → stack → Prop := 
+inductive ieval : inst → stack → stack → Prop where
   | I_Const: forall (n : Int) (s : stack),
     ieval (.Const n) s (n :: s)
   | I_Binop: forall (op : binop) (x y : Int) (s : stack),
     ieval (.Binop op) (x :: y :: s) ((bo_eval op x y) :: s)
 
+-- Determinism of a single evaluation step
 theorem ieval_determ {i s s1 s2} (hl : ieval i s s1) (hr: ieval i s s2):
   s1 = s2 :=
   by
@@ -33,4 +75,40 @@ theorem ieval_determ {i s s1 s2} (hl : ieval i s s1) (hr: ieval i s s2):
     | I_Binop op x y s' => cases hr with
       | _ => rfl
 
-  
+inductive seval : List inst → stack → stack → Prop where
+  | NilI s:
+    seval [] s s
+  | ConsI i is s0 s1 s2:
+    ieval i s0 s1 → seval is s1 s2 → seval (i :: is) s0 s2
+
+theorem seval_determ {i s s1 s2} (hl : seval i s s1) (hr : seval i s s2):
+  s1 = s2 :=
+  by induction hl generalizing s2 with
+  | NilI s => cases hr with
+    | NilI s => rfl
+  | ConsI i'  is' s' s1' s2' heval _hseval ih => cases hr with
+    | ConsI i'' is'' s'' s1'' s2'' heval' hseval' =>
+      have h1 : s1' = s1'' := by
+        apply ieval_determ
+        exact heval
+        exact heval'
+      subst h1
+      have h2 : s2' = s2 := ih hseval'
+      subst h2
+      rfl
+
+theorem stack_ex1:
+  seval [(.Const 10), (.Const 80), (.Binop .B_Div)] empty_stack [8] :=
+  by
+    apply seval.ConsI
+    { apply ieval.I_Const }
+    apply seval.ConsI
+    { apply ieval.I_Const }
+    apply seval.ConsI
+    { apply ieval.I_Binop }
+    have h: (bo_eval .B_Div 80 10) = 8 :=
+      by
+      unfold bo_eval
+      simp
+    rw [h]
+    apply seval.NilI
